习题2.2（A）：9（3、4），10，11，13，14（3、5），18（3、5），19，（B）3，6，习题2.3：（A）3（3、7），5（3），习题2.4：（A）6，9，11


# 2.2 (A)

# 9.

## (3)

$$
\begin{aligned}
f^{(50)}(x)&= \displaystyle\sum_{k=0}^{50} C_{50}^k(x^2)^{(k)}(\sin 2x)^{(50-k)} \\
&= C_{50}^0x^2(\sin 2x)^{(50)}+C_{50}^1(x^2)'(\sin 2x)^{(49)}+C_{50}^2(x^2)''(\sin 2x)^{(48)} \\
&= -2^{50}x^2\sin 2x+100\times 2^{49}x(\sin 2x)^{(49)}+2450\times2^{48}\sin 2x \\
\end{aligned}
$$

## (4)

$\because f(x)=\displaystyle\frac{1}{x^2-3x+2}=\frac{1}{(x-1)(x-2)}=\frac{1}{x-2}-\frac{1}{x-1}$

$\therefore f^{(n)}(x)=\displaystyle\frac{(-1)^nn!}{(x-2)^{n+1}}-\frac{(-1)^nn!}{(x-1)^{n+1}}$


# 10.

$\because f(x)=x(x-1)(x-2)\cdots(x-n)\quad (n\in \mathbb{N^+})$

$\therefore f'(0)=(-1)^nn!$

$将f(x)展开得f(x)=x^{n+1}+a_nx^{n}+a_{n-1}x^{n-1}+\cdots+a_0$

$\therefore f^{(n+1)}=1$


# 11.

$当n=1时,$

$\displaystyle
f'_-(0)=\lim_{x\to 0^-}\frac{f(x)-f(0)}{x-0}=\lim_{x\to 0^-}\frac{3x^3+x^2(-x)}{x}=0
$
$\displaystyle
f'_+(0)=\lim_{x\to 0^+}\frac{f(x)-f(0)}{x-0}=\lim_{x\to 0^+}\frac{3x^3+x^2(x)}{x}=0
$

$\because f'_-(0)=f'_+(0)$

$\therefore f'(0)存在, f'(x)存在, f'(x)=9x^2+2x|x|$

$当n=2时,$

$\displaystyle
f''_-(0)=\lim_{x\to 0^-}\frac{f'(x)-f(0)}{x-0}=\lim_{x\to 0^-}\frac{9x^2+2x(-x)}{x}=0
$
$\displaystyle
f''_+(0)=\lim_{x\to 0^+}\frac{f'(x)-f(0)}{x-0}=\lim_{x\to 0^+}\frac{9x^2+2x(x)}{x}=0
$

$\because f''_-(0)=f''_+(0)$

$\therefore f''(0)存在, f''(x)存在, f''(x)=18x+2|x|$

$当n=3时,$

$\displaystyle
f'''_-(0)=\lim_{x\to 0^-}\frac{f''(x)-f(0)}{x-0}=\lim_{x\to 0^-}\frac{18x+2(-x)}{x}=16
$
$\displaystyle
f'''_+(0)=\lim_{x\to 0^+}\frac{f''(x)-f(0)}{x-0}=\lim_{x\to 0^+}\frac{18x+2x}{x}=20
$

$\because f''_-(0)\neq f''_+(0)$

$\therefore f'''(0)不存在$

$\therefore f^{(n)}(0)存在的最高阶数n为2$


# 13.

$$
\begin{aligned}
F'(x)=\lim_{t\to\infty}\{t^2[f'(x+\frac{\pi}{t})-f'(x)]\sin\frac{x}{t}+t[f(x+\frac{\pi}{t})-f(x)]\cos\frac{x}{t}\}
\end{aligned}
$$


# 14.

## (3)

$\because e^{x+y}+\cos(xy)=0$

$\therefore {\rm d}(e^{x+y}+\cos(xy))=0$

$\therefore {\rm d}e^{x+y}+{\rm d}\cos(xy)=0$

$\therefore e^{x+y}{\rm d}(x+y)-\sin(xy){\rm d}(xy)=0$

$\therefore e^{x+y}{\rm d}x+e^{x+y}{\rm d}y-y\sin(xy){\rm d}x+x\sin(xy){\rm d}y=0$

$\therefore [e^{x+y}+x\sin(xy)]{\rm d}y=[y\sin(xy)-e^{x+y}]{\rm d}x$

$\therefore \displaystyle\frac{{\rm d}y}{{\rm d}x}=\frac{y\sin(xy)-e^{x+y}}{x\sin(xy)+e^{x+y}}$

