习题2.2（A）：9（3、4），10，11，13，14（3、5），18（3、5），19，（B）3，6，习题2.3：（A）3（3、7），5（3），习题2.4：（A）6，9，11


# 2.2 (A)

# 9.

## (3)

$$
\begin{aligned}
f^{(50)}(x)&= \displaystyle\sum_{k=0}^{50} C_{50}^k(x^2)^{(k)}(\sin 2x)^{(50-k)} \\
&= C_{50}^0x^2(\sin 2x)^{(50)}+C_{50}^1(x^2)'(\sin 2x)^{(49)}+C_{50}^2(x^2)''(\sin 2x)^{(48)} \\
&= -2^{50}x^2\sin 2x+100\times 2^{49}x(\sin 2x)^{(49)}+2450\times2^{48}\sin 2x \\
&= -2^{50}x^2\sin 2x+100\times 2^{49}x(\sin 2x)^{(49)}+2450\times2^{48}\sin 2x \\
\end{aligned}
$$

## (4)

$\because f(x)=\displaystyle\frac{1}{x^2-3x+2}=\frac{1}{(x-1)(x-2)}=\frac{1}{x-2}-\frac{1}{x-1}$

$\therefore f^{(n)}(x)=\displaystyle\frac{(-1)^nn!}{(x-2)^{n+1}}-\frac{(-1)^nn!}{(x-1)^{n+1}}$


# 10.

$\because f(x)=x(x-1)(x-2)\cdots(x-n)\quad (n\in \mathbb{N^+})$

$\therefore f'(0)=(-1)^nn!$

$将f(x)展开得f(x)=x^{n+1}+a_nx^{n}+a_{n-1}x^{n-1}+\cdots+a_0$

$\therefore f^{(n+1)}=1$


# 11.

$当n=1时,$

$\displaystyle
f'_-(0)=\lim_{x\to 0^-}\frac{f(x)-f(0)}{x-0}=\lim_{x\to 0^-}\frac{3x^3+x^2(-x)}{x}=0
$
$\displaystyle
f'_+(0)=\lim_{x\to 0^+}\frac{f(x)-f(0)}{x-0}=\lim_{x\to 0^+}\frac{3x^3+x^2(x)}{x}=0
$

$\because f'_-(0)=f'_+(0)$

$\therefore f'(0)存在, f'(x)存在, f'(x)=9x^2+2x|x|$

$当n=2时,$

$\displaystyle
f''_-(0)=\lim_{x\to 0^-}\frac{f'(x)-f(0)}{x-0}=\lim_{x\to 0^-}\frac{9x^2+2x(-x)}{x}=0
$
$\displaystyle
f''_+(0)=\lim_{x\to 0^+}\frac{f'(x)-f(0)}{x-0}=\lim_{x\to 0^+}\frac{9x^2+2x(x)}{x}=0
$

$\because f''_-(0)=f''_+(0)$

$\therefore f''(0)存在, f''(x)存在, f''(x)=18x+2|x|$

$当n=3时,$

$\displaystyle
f'''_-(0)=\lim_{x\to 0^-}\frac{f''(x)-f(0)}{x-0}=\lim_{x\to 0^-}\frac{18x+2(-x)}{x}=16
$
$\displaystyle
f'''_+(0)=\lim_{x\to 0^+}\frac{f''(x)-f(0)}{x-0}=\lim_{x\to 0^+}\frac{18x+2x}{x}=20
$

$\because f''_-(0)\neq f''_+(0)$

$\therefore f'''(0)不存在$

$\therefore f^{(n)}(0)存在的最高阶数n为2$


# 13.

$$
\begin{aligned}
F'(x)=\lim_{t\to\infty}\{t^2[f'(x+\frac{\pi}{t})-f'(x)]\sin\frac{x}{t}+t[f(x+\frac{\pi}{t})-f(x)]\cos\frac{x}{t}\}
\end{aligned}
$$


# 14.

## (3)

$\because e^{x+y}+\cos(xy)=0$

$\therefore {\rm d}(e^{x+y}+\cos(xy))=0$

$\therefore {\rm d}e^{x+y}+{\rm d}\cos(xy)=0$

$\therefore e^{x+y}{\rm d}(x+y)-\sin(xy){\rm d}(xy)=0$

$\therefore e^{x+y}{\rm d}x+e^{x+y}{\rm d}y-y\sin(xy){\rm d}x+x\sin(xy){\rm d}y=0$

$\therefore [e^{x+y}+x\sin(xy)]{\rm d}y=[y\sin(xy)-e^{x+y}]{\rm d}x$

$\therefore \displaystyle\frac{{\rm d}y}{{\rm d}x}=\frac{y\sin(xy)-e^{x+y}}{x\sin(xy)+e^{x+y}}$

## (5)

$\because y=\sin(x+y)$

$\therefore {\rm d}y={\rm d}\sin(x+y)$

$\therefore [1-\cos(x+y)]{\rm d}y=\cos(x+y){\rm d}x$

$\therefore [1-\cos(x+y)]{\rm d}^2y+2\sin(x+y){\rm d}x{\rm d}y+\sin(x+y){\rm d}y^2+\sin(x+y){\rm d}x^2=0$

$\therefore\displaystyle [1-\cos(x+y)]\frac{{\rm d}^2y}{{\rm d}x^2}+2\sin(x+y)\frac{{\rm d}y}{{\rm d}x}+\sin(x+y)\frac{{\rm d}y^2}{{\rm d}x^2}+\sin(x+y)=0$

$\therefore\displaystyle [1-\cos(x+y)]\frac{{\rm d}^2y}{{\rm d}x^2}+2\sin(x+y)\frac{{\rm d}y}{{\rm d}x}+\sin(x+y)\frac{{\rm d}y^2}{{\rm d}x^2}+\sin(x+y)=0$

$\because\displaystyle \frac{{\rm d}y}{{\rm d}x}=\frac{\cos(x+y)}{1-\cos(x+y)}$

$\therefore\displaystyle [1-\cos(x+y)]\frac{{\rm d}^2y}{{\rm d}x^2}+2\sin(x+y)\frac{\cos(x+y)}{1-\cos(x+y)}+\sin(x+y)[\frac{\cos(x+y)}{1-\cos(x+y)}]^2+\sin(x+y)=0$

$\therefore\displaystyle \frac{{\rm d}^2y}{{\rm d}x^2}=-\frac{\sin(x+y)}{[1-\cos(x+y)]^3}$


# 18.

## (3)

$当a=0时,$

$\therefore x=0,y=0$

$\therefore \displaystyle \frac{{\rm d}y}{{\rm d}x}\bigg|_{t=2}=\frac{{\rm d}y}{{\rm d}x}\bigg|_{x=0}=0$

$当a\neq 0时,$

$\therefore\displaystyle \frac{{\rm d}y}{{\rm d}x}\bigg|_{t=2}=\frac{\displaystyle\frac{{\rm d}y}{{\rm d}t}\bigg|_{t=2}}{\displaystyle\frac{{\rm d}x}{{\rm d}t}\bigg|_{t=2}}=\frac{\displaystyle\frac{2a(1+t^2)-4at^2}{(1+t^2)^2}\bigg|_{t=2}}{\displaystyle\frac{6at(1+t^2)-6at^3}{(1+t^2)^2}\bigg|_{t=2}}=\frac{10a-16a}{60a-48a}=-\frac{1}{2}$

## (5)

$\therefore\displaystyle \frac{{\rm d}^2y}{{\rm d}x^2}=\frac{\displaystyle\frac{{\rm d}^2y}{{\rm d}t^2}}{\displaystyle\frac{{\rm d}x}{{\rm d}t}\cdot\frac{{\rm d}x}{{\rm d}t}}=\frac{(tf(t)-f(t))''}{f'(t)\cdot f'(t)}=\frac{2f'(t)+(t-1)f''(t)}{[f'(t)]^2}$


# 19.

$\because \Gamma: r=r(\theta), x=r(\theta)\cos\theta, x=r(\theta)\sin\theta$

$\therefore\displaystyle k=\frac{{\rm d}y}{{\rm d}x}=\frac{\displaystyle\frac{{\rm d}y}{{\rm d}\theta}}{\displaystyle\frac{{\rm d}x}{{\rm d}\theta}}=\frac{r'(\theta)\sin\theta+r(\theta)\cos\theta}{r'(\theta)\cos\theta-r(\theta)\sin\theta}$

$对于心型线r(\theta)=a(1-\cos\theta),r'(\theta)=a\sin\theta$

$
\begin{aligned}
\therefore\displaystyle k&=\frac{a\sin^2\theta+a(1-\cos\theta)\cos\theta}{a\sin\theta\cos\theta-a(1-\cos\theta)\sin\theta} \\
&=\frac{a\sin^2\theta-a\cos^2\theta+a\cos\theta}{2a\sin\theta\cos\theta-a\sin\theta} \\
&=\frac{-a\cos2\theta+a\cos\theta}{a\sin2\theta-a\sin\theta} \\
\end{aligned}
$


# 2.2 (B)

# 3.

$\therefore f'_-(0)=\displaystyle\lim_{x\to 0^-}\frac{\frac{1}{x}(1-\cos ax)-0}{x-0}=\lim_{x\to 0^-}{\frac{1}{x^2}\cdot\frac{1}{2}(ax)^2}=\frac{a^2}{2}$

$\quad f'_+(0)=\displaystyle\lim_{x\to 0^+}\frac{\frac{1}{x}\ln(b+x^2)-0}{x-0}=\lim_{x\to 0^+}\frac{1}{x^2}\ln(b+x^2)$

$\therefore 只有b=1时, f'_+(0)才存在, 且f'_+(0)=1$

$\therefore f'_-(0)=f'_+(0)=\displaystyle\frac{a^2}{2}=1$

$\therefore a=\sqrt{2}$

$
\therefore f'(x)=
\begin{cases}
\displaystyle\frac{\sqrt{2}x\sin\sqrt{2}x+\cos\sqrt{2}x-1}{x^2} ,&x<0 \\
1, &x=0 \\
\displaystyle\frac{2}{x^2+1}-\frac{1}{x^2}\ln(x^2+1) ,&x>0 \\
\end{cases}
$


# 6.

$当x<1时, n\to\infty, e^{n(x-1)}\to 0$

$\therefore f(x)=ax+b$

$当x=1时, n\to\infty, e^{n(x-1)}=1$

$\therefore f(x)=\displaystyle\frac{x^2+ax+b}{2}$

$当x>1时, n\to\infty, e^{n(x-1)}=\infty$

$\therefore f(x)=x^2$

$
\therefore
f(x)=
\begin{cases}
ax+b, &x<1 \\
\displaystyle\frac{x^2+ax+b}{2}, &x=1 \\
x^2, &x>1 \\
\end{cases}
$

$对于连续性:$

$\because f(1+0)=1$

$\therefore f(1-0)=a+b=1, f(1)=\displaystyle\frac{a+b+1}{2}=1$

$\therefore a+b=1$

$对于可导性:$

$\therefore f'_+(1)=\displaystyle\lim_{\Delta x\to 0^+}\frac{(1+\Delta x)^2-1}{\Delta x}=\lim_{\Delta x\to 0^+}\frac{\Delta x^2+2\Delta x}{\Delta x}=2$

$\therefore f'_-(1)=\displaystyle\lim_{\Delta x\to 0^-}\frac{a(1+\Delta x)+b-1}{\Delta x}=2$

$\therefore a=2,b=-1$

$
\therefore
f(x)=
\begin{cases}
2x-1, &x<1 \\
\displaystyle\frac{x^2+2x-1}{2}, &x=1 \\
x^2, &x>1 \\
\end{cases}
$

$
\therefore
f(x)=
\begin{cases}
2, &x\leq 1 \\
2x, &x>1 \\
\end{cases}
$

# 2.3 (A)

# 3.

## (3)

$
\begin{aligned}
{\rm d}y&={\rm d}[e^{-x}\cos(3-x)] \\
&=\cos(3-x){\rm d}e^{-x}+e^{-x}{\rm d}\cos(3-x) \\
&=[\sin(3-x)-\cos(3-x)]e^{-x}{\rm d}x \\
\end{aligned}
$

## (7)

$\because y=\displaystyle\sqrt[3]{\frac{1-x}{1+x}}$

$\therefore\displaystyle \ln y=\frac{1}{3}\ln(1-x)-\frac{1}{3}\ln(1+x)$

$\therefore\displaystyle \frac{y'}{y}=\frac{1}{3x-3}-\frac{1}{3x+3}$

$\therefore\displaystyle {\rm d}y=y'{\rm d}x=(\frac{1}{3x-3}-\frac{1}{3x+3})\sqrt[3]{\frac{1-x}{1+x}}{\rm d}x$

# 5.(3)

$\because f(x)\approx f(x_0)+f'(x_0)(x-x_0)$

$取x_0=25$

$\therefore \sqrt{25.4}\approx \sqrt{25}+\displaystyle\frac{(25.4-25)}{2\sqrt{25}}=5+\frac{0.4}{10}=5.04$


# 2.4 (A)

# 6.

$\because f为奇函数$

$\therefore f(a)=-f(-a)$

$当a>0时,$

$\therefore 由拉格朗日中值定理知$

$\quad \exist\xi\in (-a,a), f'(\xi)=\displaystyle\frac{f(a)-f(-a)}{a-(-a)}=\frac{f(a)}{a}$

$当a<0时, 同理可知也成立$

$\therefore \forall a\neq 0, 必定存在\xi在-a和a之间, 使得f'(\xi)=\displaystyle\frac{f(a)}{a}$

# 9.

$令F(x)=\arcsin x+\arccos x$

$假设F(x_0)\neq \displaystyle\frac{\pi}{2}$

$\because\displaystyle F(-1)=\frac{\pi}{2}$

$\therefore 由Lagrange定理可知\exist\xi\in(-1,x_0), F'(\xi)=\displaystyle\frac{F(x_0)-F(-1)}{\xi+1}\neq 0$

$\because F'(x)=\displaystyle\frac{1}{\sqrt{1-x^2}}-\frac{1}{\sqrt{1-x^2}}=0$

$\therefore 产生矛盾$

$\therefore\displaystyle F(x)=\frac{\pi}{2}$

# 11.

$令F(x)=e^xf(x), x_1和x_2是f(x)的两个零点$

$\therefore F(x_1)=F(x_2)=e^xf(x_1)=e^xf(x_2)=0$

$\because f(x)可微$

$\therefore \exist\xi\in(x_1,x_2), F'(\xi)=e^{\xi}f(\xi)+e^{\xi}f'(\xi)=0$

$\therefore \exist\xi\in(x_1,x_2), f(\xi)+f'(\xi)=0$