# Practice 5

## 1.

$
\begin{aligned}
I_n&=\int \sin^nx{\rm d}x \\
&=\int \sin^{n-1}x{\rm d}(-\cos x) \\
&=-\cos x\sin^{n-1} + \int \cos x{\rm d}\sin^{n-1}x \\
&=-\cos x\sin^{n-1} + \int \cos^2 x(n-1)\sin^{n-2}x{\rm d}x \\
&=-\cos x\sin^{n-1} + (n-1)\int (1-\sin^2 x)\sin^{n-2}x{\rm d}x \\
&=-\cos x\sin^{n-1} + (n-1)(I_{n-2}-I_n) \\
\end{aligned}
$

$I_n=\displaystyle\frac{1}{n}\cos x\sin^{n-1}x+\frac{n-1}{n}I_{n-2}, \quad n\geq 2$


## 2.

$x^2-1=\tan^2 t, x=\sec t$
$x^2+1=\sec^2 t, x=\tan t$

$a>0$

$\displaystyle\sin t=2\sin\frac{t}{2}\cos\frac{t}{2}=\frac{2\sin\frac{t}{2}\cos\frac{t}{2}}{\sin^2\frac{t}{2}+\cos^2\frac{t}{2}}=\frac{2\tan \frac{t}{2}}{\tan^\frac{t}{2}+1}$

$
\begin{aligned}
\int\frac{{\rm d}x}{\sqrt{x^2+a^2}} &= \int\frac{{\rm d}a\tan t}{\sqrt{a^2\sec^2t}} \\
&=\int\frac{a\sec^2 t{\rm d}t}{a\sec t} \\
&=\int\sec t{\rm d}t \\
&=\int\frac{{\rm d}t}{\cos t} \\
&=\int\frac{\cos^2\frac{t}{2}+\sin^2\frac{t}{2}}{\cos^2\frac{t}{2}-\sin^2\frac{t}{2}}{\rm d}t \\
&=\int\frac{\tan^2\frac{t}{2}+1}{1-\tan^2\frac{t}{2}}{\rm d}t \\
&=\int\frac{u^2+1}{1-u^2}\cdot 2\cos^2\frac{t}{2}{\rm d}u \\
&=\int\frac{u^2+1}{1-u^2}\cdot \frac{2}{1-u^2}{\rm d}u
\end{aligned}
$

$
\begin{aligned}
\int\frac{{\rm d}x}{\sqrt{x^2+a^2}} &= \int\frac{{\rm d}a\tan t}{\sqrt{a^2\sec^2t}} \\
&=\int\frac{a\sec^2 t{\rm d}t}{a\sec t} \\
&=\int\sec t{\rm d}t \\
&=\int\frac{{\rm d}t}{\cos t} \\
&=\int\frac{\cos t{\rm d}t}{\cos^2 t} \\
&=\int\frac{{\rm d}\sin t}{1-\sin^2 t} \\
&=\int(\frac{1}{1-\sin t}+\frac{1}{1+\sin t}){\rm d}\sin t \\
&=-\int\frac{1}{1-\sin t}{\rm d}(1-\sin t)+\int\frac{1}{1+\sin t}{\rm d}(1+\sin t) \\
&=-\int\frac{1}{1-\sin t}{\rm d}(1-\sin t)+\int\frac{1}{1+\sin t}{\rm d}(1+\sin t) \\
&=\ln(1+\sin t)-\ln(1-\sin t)+C \\
\end{aligned}
$


$\displaystyle\ch u=\frac{e^u+e^{-u}}{2}, \sh u=\frac{e^u-e^{-u}}{2}$

$\ch^2u-\sh^2u=1$

$\ch 2u=2\ch^2u-1=\ch^2u+\sh^2u=1+2\sh^2u$

$\sh2u=2\sh u\ch u$

$
\begin{aligned}
\int\frac{{\rm d}x}{\sqrt{x^2+a^2}} &= \int\frac{{\rm d}a\sh u}{\sqrt{a^2\ch^2u}} \\
&=\int\frac{a\ch t{\rm d}u}{a\ch u} \\
&=\int{\rm d}u \\
&=u \\
&=\sh^{-1}(\frac{x}{a}) \\
\end{aligned}
$

$
\begin{aligned}
\int\frac{{\rm d}x}{\sqrt{x^2-a^2}} =\ch^{-1}(\frac{x}{a}) \\
\end{aligned}
$

$\because x=a\displaystyle\frac{e^u+e^{-u}}{2}$

$\therefore\displaystyle e^{2u}-2\frac{x}{a}e^u-1=0$


# 3.

$倒代换$

$
\begin{aligned}
\int\frac{\sqrt{a^2-x^2}}{x^4}{\rm d}x &=\int\frac{a^2-\frac{1}{t^2}}{\frac{1}{t^4}}(-\frac{1}{t^2}){\rm d}t \\
&=\int -t\sqrt{a^2t^2-1}{\rm d}t \\
&=\int -\frac{1}{2a^2}\sqrt{a^2t^2-1}{\rm d}a^2t^2 \\
&=-\frac{1}{2a^2}\int\sqrt{u-1}{\rm d}u \\
&=-\frac{1}{2a^2}\int{(u-1)^\frac12}{\rm d}(u-1) \\
&=-\frac{1}{3a^2}{(u-1)^\frac32}+C \\
\end{aligned}
$


# 4.

$\displaystyle\int\frac{A\sin x+B\cos x}{C\sin x+D\cos x}{\rm d}x=mx+n\displaystyle\int\frac{{\rm d}(C\sin x+D\cos x)}{C\sin x+D\cos x}$

$A\sin x+B\cos x=m(C\sin x+D\cos x)+n(C\cos x-D\sin x)$

$\begin{vmatrix}C&-D\\D&C\end{vmatrix}\begin{pmatrix}m\\n\end{pmatrix}=\begin{pmatrix}A\\B\end{pmatrix}$

$用克拉默法则解$


# 5.

$\displaystyle\int\frac{P_n(x)}{Q_m(x)}{\rm d}x$

$
\begin{aligned}
\int\frac{x^4+1}{x(x^2+1)^2}{\rm d}x &= \frac{1}{2}\int\frac{x^4+1}{x^2(x^2+1)^2}{\rm d}x^2 \\
&= \frac{1}{2}\int\frac{u^2+1}{u(u+1)^2}{\rm d}u \\
\end{aligned}
$

$\displaystyle\frac{A}{u}+\frac{Cu+D}{(u+1)^2}=\frac{u^2+1}{u(u+1)^2}$

$
\begin{cases}
A(u+1)^2+(Cu+D)u=u^2+1 \\
(A+C)u^2+(2A+D)u+A=u^2+1
\end{cases}
$


# 6.

$\sin u=\sqrt{x}, \sin^2u=x$

$
\begin{aligned}
\int\frac{\arcsin\sqrt{x}}{\sqrt{1-x}}{\rm d}x &= \int\frac{u}{\sqrt{1-sin^2u}}{\rm d}\sin^2u \\
&=\int\frac{u\cdot 2\sin u\cos u{\rm d}u}{\cos u} \\
&=2\int u\sin u{\rm d}u \\
&=2\int u{\rm d}(-\cos u) \\
&=-2u\cos u+2\int\cos u{\rm d}u \\
&=-2u\cos u+2\sin u + C \\
&=-2\arcsin\sqrt{x}\sqrt{1-x}+2\sqrt{x} + C \\
\end{aligned}
$

$$
\begin{aligned}
\int\frac{\arcsin\sqrt{x}}{\sqrt{1-x}}{\rm d}x &=-\int\frac{\arcsin\sqrt{x}}{\sqrt{1-x}}{\rm d}(1-x) \\
&=-2\int\arcsin\sqrt{x}{\rm d}\sqrt{1-x} \\
&=-2\sqrt{1-x}\arcsin\sqrt{x}+2\int\sqrt{1-x}{\rm d}\arcsin\sqrt{x} \\
&=-2\sqrt{1-x}\arcsin\sqrt{x}+2\int\sqrt{1-x}\cdot \frac{1}{\sqrt{1-x}}\cdot \frac{1}{2\sqrt{x}}{\rm d}x \\
&=-2\sqrt{1-x}\arcsin\sqrt{x}+\int\frac{1}{\sqrt{x}}{\rm d}x \\
&=-2\sqrt{1-x}\arcsin\sqrt{x}+2\sqrt{x}+C \\
\end{aligned}
$$


# 7.

$
\begin{aligned}
\sin^2x\cos^4x{\rm d}x &= \int\sin^2x\cos^6x{\rm d}\tan x \\
&=\int\frac{\sin^2x\cos^6x}{(\sin^2x+\cos^2x)^4}{\rm d}\tan x \\
\end{aligned}
$

$
\begin{aligned}
\sin^2x\cos^4x{\rm d}x &= \int\frac{1-\cos2x}{2}(\frac{1+\cos2x}{2})^2{\rm d}x \\
&=\frac{1}{8}\int(1+\cos2x-\cos^22x-\cos^32x){\rm d}x \\
\end{aligned}
$


# 8.

$
\begin{aligned}
I&=\int\frac{e^{\arctan x}}{(1+x^2)^\frac{3}{2}}{\rm d}x \\
&=\int\frac{e^t}{\sec^3t}\sec^2t{\rm d}t \\
\end{aligned}
$