![](./images/2020-12-25-08-03-00.png)

![](./images/2020-12-25-08-03-15.png)

[(1)](./H6.md)

$$
\begin{aligned}
\frac{e-(1+x)^\frac{1}{x}}{x}
&=\frac{e-e^{\frac{1}{x}\ln(x+1)}}{x} \\
\end{aligned}
$$

[(2)](./H6.md)

# 区间再现

$沿着区间中轴翻转, 面积不变$

$\displaystyle\int_a^bf(t){\rm d}t=\int_a^bf(a+b-t){\rm d}t=\frac{1}{2}\int_a^b[f(t)+f(a+b-t)]{\rm d}t$


$也可以写成$

$\displaystyle\int_a^bf(t){\rm d}t=\int_a^{\frac{a+b}{2}}[f(t)+f(a+b-t)]{\rm d}t$

## 例题一

$\displaystyle\int_0^{\pi}\frac{x\sin x}{1+\cos^2x}{\rm d}x=\frac{1}{2}\int_0^{\pi}[\frac{x\sin x}{1+\cos^2x}+\frac{(\pi-x)\sin (\pi-x)}{1+\cos^2x}]{\rm d}x$

## 例题二

$$
\begin{aligned}
\int_0^{\frac{\pi}{4}}\ln(1+\tan x){\rm d}x
&=\frac{1}{2}\int_0^{\frac{\pi}{4}}[\ln(1+\tan x)+\ln(1+\tan (\frac{\pi}{4}-x))]{\rm d}x \\
&=\frac{1}{2}\int_0^{\frac{\pi}{4}}[\ln(1+\tan x)+\ln(1+\frac{1-\tan x}{1+\tan x})]{\rm d}x \\
&=\frac{\pi}{8}\ln 2
\end{aligned}
$$

## 例题三

$$
\begin{aligned}
\int_0^\frac{\pi}{4}\frac{x{\rm d}x}{\cos(\frac{\pi}{4}-x)\cos x}
&=\frac{1}{2}\int_0^\frac{\pi}{4}\frac{x+\frac{\pi}{4}-x}{\cos(\frac{\pi}{4}-x)\cos x}{\rm d}x \\
\end{aligned}
$$

## 例题四

$$
\begin{aligned}
\int_0^\pi xf(\sin x){\rm d}x
&=\frac{1}{2}\int_0^\pi (x+\pi-x)f(\sin x){\rm d}x \\
&=\frac{\pi}{2}\int_0^\pi f(\sin x){\rm d}x \\
\end{aligned}
$$


# 华利兹公式

$$
\begin{aligned}
I_n
&=\int_0^{\frac{\pi}{2}}\sin^nx{\rm d}x \\
&=\frac{n-1}{n}\cdot\frac{n-3}{n-2}\cdot\cdots\cdot\frac{1}{2}\cdot \frac{\pi}{2}, n为偶 \\
&=\frac{n-1}{n}\cdot\frac{n-3}{n-2}\cdot\cdots\cdot\frac{4}{5}\cdot \frac{2}{3}\cdot \pi, n为奇 \\
\end{aligned}
$$


# 用定积分求无穷级数

$$
\begin{aligned}
\displaystyle(b^\frac{1}{n}-1)\sum_{i=0}^nb^\frac{i}{n}\sin\frac{2n+i}{2n}
&=\sum_{i=0}^n(b^\frac{i+1}{n}-b^{\frac{i}{n}})\sin(\frac{\frac{i}{n}+\frac{i+1}{n}}{2}) \\
&=\int_1^b\sin x{\rm d}x \\
&=\cos 1-\cos b
\end{aligned}
$$

# 反常积分

$$
\begin{aligned}
\int_0^1\frac{{\rm d}x}{\sqrt{(1-x^2)(1-k^2x^2)}}
&=\int_0^1\frac{{\rm d}x}{\sqrt{1+x}\sqrt{1-x}(1-k^2x^2)} \\
\end{aligned}
$$