# 习题课

$f:\mathbb{R}^n\to \mathbb{R}, x\to f(x)$

连续:

$\forall{\rm d}(x_0,x_0)<\delta, |f(B(x_0, \delta))|<\varepsilon$

$\therefore f(B(x_0, \delta))\subset B(f(x_0), \varepsilon)$

## 定理

$f$ 连续 $\Leftrightarrow$ 开集的原像是开集 $\Leftrightarrow$ 闭集的原象是闭集

**"$\Rightarrow$":**

$\forall U\subset E$ 中的开集, $f^{-1}(U)\subset D$

想证其为开集

$\Leftrightarrow$

$\forall x_0\in f^{-1}(U), f(x_0)\in U$

$\because\exist \varepsilon, B(f(x_0), \varepsilon)\subset U$

$\therefore \exist\delta$ 满足 $f(B(x_0, \delta))\subset B(f(x_0), \varepsilon)\subset U$

$\therefore B(x_0, \delta)\subset f^{-1}(B(f(x_0), \delta))\subset f(U)$

**"$\Leftarrow$":**

$\forall\varepsilon\in\mathbb{R}_+, B(f(x), \varepsilon)\subset E$

任取 $x_0\in f^{-1}(B(f(x), \varepsilon))$, $\exist \delta, B(x_0, \delta)\subset f^{-1}(B(f(x_0), \varepsilon))$

$\therefore f(B(x_0), \delta)\subset B(f(x_0), \varepsilon)$

$\therefore f$ 是连续的


## 多元函数

$\displaystyle\lim_{(x,y)\to (0,0)}\frac{P(x,y)}{Q(x,y)}=\frac{a_1x^my^0+\cdots }{b_1x^ny^0+\cdots }$

当 $m\leq n$, 极限不存在.

当 $m>n$,

1. $\begin{cases}Q(1,y)=0 \\Q(x,1)=0 \\\end{cases}$ 均无实根, 那么$\displaystyle \lim_{(x,y)\to (0,0)}\frac{P}{Q}=0$
2. 否则极限不存在.


## 例题

### 1.

令 $x=\rho\cos\theta, y=\rho\sin\theta$

$\displaystyle\lim_{(x,y)\to (0,0)}f(x,y)=xy\sin\frac{1}{x^2+y^2}=\lim_{\rho\to 0}\rho^2\sin\theta\cos\theta\sin\frac{1}{\rho^2}=0$

$\displaystyle A=f_x(0,0)=\lim_{x\to 0}\frac{f(x, 0)-f(0,0)}{x}=0$

$\displaystyle B=f_y(0,0)=\lim_{y\to 0}\frac{f(0, y)-f(0,0)}{y}=0$

$\displaystyle \lim_{(\Delta x,\Delta y)\to (0,0)}\frac{\Delta f-A\Delta x-B\Delta y}{\sqrt{\Delta x^2+\Delta y^2}}=\frac{\Delta x\Delta y\sin\frac{1}{\Delta x^2+\Delta y^2}}{\sqrt{\Delta x^2+\Delta y^2}}\leq \frac{\Delta x\Delta y}{\sqrt{\Delta x^2+\Delta y^2}}$

带入上定理: $\sqrt{1+\Delta y^2}=0, \sqrt{1+\Delta x^2}=0$ 均无实根

$\therefore$ 极限为零, 可微.

### 隐函数求导

$u=(x,y), v=v(x,y)$

$F(x,y,u,v)=0, G(x,y,u,v)=0$

$\therefore\displaystyle F_x+\frac{\partial u}{\partial x}F_u+\frac{\partial v}{\partial x}F_v=0$

$\therefore\displaystyle G_x+\frac{\partial u}{\partial x}G_u+\frac{\partial v}{\partial x}G_v=0$

记 $\displaystyle J=\frac{\partial (F,G)}{\partial (u,v)}=\begin{vmatrix}F_u&F_v\\G_u&G_v\end{vmatrix}$

$\displaystyle \frac{\partial (F,G)}{\partial (x,v)}=\begin{vmatrix}F_x&F_v\\G_x&G_v\end{vmatrix}$

$\therefore \displaystyle\frac{\partial u}{\partial x}=-\frac{1}{J}\frac{\partial (F,G)}{\partial (x,v)}$

$\therefore \displaystyle\frac{\partial v}{\partial x}=-\frac{1}{J}\frac{\partial (F,G)}{\partial (u,x)}$

### 4.

$\because F(x,y,z)=0$

<!-- $\therefore\displaystyle F_x+\frac{\partial y}{\partial x}F_y+\frac{\partial z}{\partial x}$ -->

$\because\displaystyle J=\begin{vmatrix}F_y&F_z\\G_y&G_z\end{vmatrix}=\begin{vmatrix}F_y&F_z\\-xf''&1\end{vmatrix}=F_y+xf' F_z$

$\quad\displaystyle \frac{\partial (F,G)}{\partial (y,x)}=\begin{vmatrix}F_y&F_x\\-xf'&f+xf'\end{vmatrix}=F_y(f+xf')-xf' F_x$

$\therefore\displaystyle \frac{{\rm d}z}{{\rm d}x}=-\frac{1}{J}\frac{\partial (F,G)}{\partial (y,x)}$

### 5.

**"$\Leftarrow$":**

取 $t=1$,

$kF(x,y,z)=kF(tx,ty,tz)$

**"$\Rightarrow$":**

$\because$ 要证 $F(tx,ty,tz)=t^kF(x,y,z)$

$\therefore$ 即证 $\displaystyle \varphi(t)=\frac{F(tx, ty, tz)}{t^k}=F(x,y,z)=\varphi(1)$

$\therefore\displaystyle \varphi'(t)=-\frac{k}{t^{k+1}}F(tx, ty, tz)+\frac{1}{t^{k+1}}(txF_x(tx, ty, tz)+tyF_y(tx, ty, tz)+tzF_z(tx, ty, tz))=0$

$\therefore \varphi(t)=\varphi(1)$