# 作业

![](2020-10-12-09-42-17.png)

# 习题一

## 1.1

                    1/3     -7/9
            3       -2      1
    ----------------------------
    1       -3      -1      -1
    1       -2/3    1/3 
    ----------------------------
            -7/3    -4/3    -1
            -7/3    14/9    -7/9
            --------------------
                    -26/9   -2/9

$$
q(x)=\frac{1}{3}x - \frac{7}{9}, r(x)=-\frac{26}{9} x -\frac{2}{9}
$$

## 2.2

                    1       -m      m*m+p-1
                    1       m       1
    -------------------------------------------
    1       0       p       0       q
    1       m       1
    -------------------------------------------
            -m      p-1     0       q
            -m      -m*m    -m
            -----------------------------------
                    m*m+p-1 m           q
                    m*m+p-1 m(m^2+p-1)  m*m+p-1
                    -----------------------------
                            2m-m^3-pm   q-p-m^2+1

$$
q(x)=x^2-mx+m^2+p-1
$$

$$
r(x)=(2m-m^3-pm)x+q-p-m^2+1
$$

要能整除, 则说明

$$
\begin{cases}
    &2m-m^3-pm = 0 \\
    &q-p-m^2+1 = 0 \\
\end{cases}
$$

$$
\begin{cases}
    &m^2+p = 2 \\
    &q=1 \\
\end{cases}
或
\begin{cases}
    &m = 0 \\
    &p-q=1 \\
\end{cases}
$$

## 3

### 1)

        2   -6  13  -39 109
                    1   3
    2   0   -5  0   -8  0
    ----------------------
    2   0
    2   6
    ------
        -6  -5
        -6  -18
        -------
            13  0
            13  39
            ------
                -39 -8
                -39 -117
                --------
                    109 0
                    109 327
                    -------
                        -327

$$
q(x) = 2x^4-6x^3+13x^2-39x+109, r(x)=-327
$$

### 2)

            1       -2i     -5-2i
                    1       -1+2i
    1       -1      -1      0
    -----------------------------
    1       -1
    1       -1+2i
    -------------
            -2i     -1
            -2i     2i+4
            -------------
                    -5-2i   0
                    -5-2i   (-1+2i)(-5-2i)=5+4-10i+2i=9-8i

$$
q(x)=x^2-2ix-5-2i)
$$