![](2020-10-14-18-38-42.png)

# 5.2

                1       -1  |               -1/3    10/9    |   
        1   -3  0       1   |       -3      -1      2       |
    ----------------------  |   --------------------------  |
    1   -4  0   0       1   |   1   -3      0       1       |
    1   -3  0   1           |   1   1/3     -2/3            |
    --------------          |   --------------------------  |
        -1  0   -1      1   |       -10/3   2/3     1       |
        -1  3   0       -1  |       -10/3   -10/9   20/9    |
        ------------------  |   --------------------------  |
            -3  -1      2   |               16/9    -11/9   |
            -3  33/16
            --------------
                -49/16  2
                149/16  539/256
                ---------------
                        -27/256

所以最大公因式是1.

# 6.2

$q_1=2x$

$q_2=-\displaystyle\frac{1}{3}x+\frac{1}{3}$

$q_3=6x+9$

            2       -1      -5      4
    ----------------------------------
    4       -2      -16     5       9
    4       -2      -10     8
    ----------------------------------
                    -6      -3      9

            -6      -3      9
    --------------------------
    2       -1      -5      4
    2       1       -3
    --------------------------
            -2      -2      4
            -2      -1      3
            ------------------
                    -1      1

            -1      1
    -------------------
    -6      -3      9
    -6      6
    ------------------
            -9      9
            -9      9
            ----------
                    0


$$
\begin{aligned}
x-1=-r_2&=g(x)+q_2(x)f(x)-q_1(x)q_2(x)g(x) \\
&=q_2(x)f(x)+(1-q_1(x)q_2(x))g(x)
\end{aligned}
$$

$\therefore u(x)=q_2(x)=-\displaystyle\frac{1}{3}x+\frac{1}{3}$

$\therefore v(x)=1-2x(-\displaystyle\frac{1}{3}x+\frac{1}{3})=\frac{2}{3}x^2-\frac{2}{3}x+1$


# 7.

    1       0       t       u
    --------------------------
    1       1+t     2       2u
    1       0       t       u
    --------------------------
            1+t     2-t     u

            1+t             2-t         u
    --------------------------------------
    1       0               t           u
    1       (2-t)/(1+t)     u/(1+t)
    --------------------------------------
            -(2-t)/(1+t)    t-u/(1+t)   u
            1+t             2-t         u
            ------------------------------
            0               0           0

$$
\begin{cases}
-2+t=(1+t)^2 \\
t-u=(2-t)(1+t)
\end{cases}
\Rightarrow
\begin{cases}
t^2+t+3=0 \\
t^2-u-2=0
\end{cases}
\Rightarrow
\begin{cases}
t =\displaystyle\frac{-1\pm 11i}{2} \\
u = \displaystyle\frac{-9\pm 11i}{2}
\end{cases}
$$

$\therefore t =\displaystyle\frac{-1\pm 11i}{2}$

$\therefore u = \displaystyle\frac{-9\pm 11i}{2}$


# 8.

