17. 20. 22. 

# 17.

$求t值使f(x)=x^3-3x^2+tx-1有重根.$

解:

$\therefore f'(x)=3x^2-6x+t$

                3           -6          t
    --------------------------------------------
    1           -3          t           -1
    1           -2          t/3
    --------------------------------------------
                -1          2t/3        -1
                -1          2           -t/3
                --------------------------------
                            2(t/3-1)      t/3-1

$当t=3时, (f(x),f'(x))=\frac{1}{3}f'(x)=(x-1)^2$

$当t\neq 3时,$

                2(t/3-1)    t/3-1
    --------------------------------
    3           -6          t
    3           3/2
    --------------------------------
                -15/2       t
                -15/2       -15/4
                --------------------
                            t+15/4=0
                
$\therefore t=-\displaystyle\frac{15}{4}$

# 20.

$\therefore f(x)=1+x+\displaystyle\frac{x^2}{2!}+\cdots+\frac{x^n}{n!}$

$\therefore f'(x)=1+x+\displaystyle\frac{x^2}{2!}+\cdots+\frac{x^{n-1}}{(n-1)!}$

$假设f(x)有重根a,则f(a)=0, f'(x)=0$

$\therefore f(a)=1+a+\displaystyle\frac{a^2}{2!}+\cdots+\frac{a^n}{n!}=0,$
$\quad f'(a)=1+a+\displaystyle\frac{a^2}{2!}+\cdots+\frac{a^{n-1}}{(n-1)!}=0$

$\therefore f(a)-f'(x)=\displaystyle\frac{a^n}{n!}=0$

$\therefore a=0$

$\therefore f(a)=f(0)=1 \neq 0, 产生矛盾$

$\therefore f(x)没有重根.$


# 22.

$证明: x_0是f(x)的k重根的充分必要条件是f(x_0)=f'(x_0)=\cdots =f^{(k-1)}(x_0)=0, 而f^{(k)}(x_0)\neq 0.$

## $\Rightarrow$:

$\because x_0是f(x)的k重根$

$\therefore (x-x_0)是f(x)的k重因式$

$\therefore (x-x_0)是f'(x)的k-1重因式$

$\cdots$

$\therefore (x-x_0)是f^{(k-1)}(x)的1重因式$

$\therefore (x-x_0)不是f^{(k)}(x)的因式$

$\therefore f(x_0)=f'(x_0)=\cdots=f^{(k-1)}(x_0)=0, f^{(k)}(x_0)\neq 0$

## $\Leftarrow$:

$\because (x-x_0)是f^{(k-1)}(x)的1重因式, (x-x_0)不是f^{(k)}(x)的因式$

$\therefore (x-x_0)|f^{(k-1)}(x), (x-x_0)|f^{(k)}(x)$