![](2020-11-26-21-04-48.png)

![](2020-11-26-21-05-00.png)

![](2020-11-26-21-05-11.png)

# 1.

## (1)

$$
\begin{aligned}
&
\begin{bmatrix}
1 &-1 &-1 &-3 \\
1 &-1 &0 &1 \\
4 &-4 &0 &0 \\
\end{bmatrix}=
\begin{bmatrix}
1 &-1 &-1 &-3 \\
0 &0 &1 &4 \\
0 &0 &4 &12 \\
\end{bmatrix}=
\begin{bmatrix}
1 &-1 &-1 &-3 \\
0 &0 &1 &4 \\
0 &0 &0 &1 \\
\end{bmatrix}
\\ &=
\begin{bmatrix}
1 &-1 &-1 &0 \\
0 &0 &1 &0 \\
0 &0 &0 &1 \\
\end{bmatrix}=
\begin{bmatrix}
1 &-1 &0 &0 \\
0 &0 &1 &0 \\
0 &0 &0 &1 \\
\end{bmatrix}
\end{aligned}
$$

$\therefore x_1-x_2=0, x_3=0, x_4=0$