P235 15. 17.


# P235

## 15.

$
\begin{aligned}
n\sum_{i=1}^nx_i^2-(\sum_{i=1}^nx_i)^2
&=(n-1)\sum_{i=1}^nx_i^2-2\sum_{1\leq i < j\leq n}^nx_ix_j \\
&=\sum_{1\leq i< j\leq n}(x_i-x_j)^2 \\
&\geq 0
\end{aligned}
$

对任意一组数 $(c_1,c_2,\cdots,c_n)$ 带入原式都有 $\displaystyle\sum_{1\leq i< j\leq n}(c_i-c_j)^2$

$\displaystyle\therefore n\sum_{i=1}^nx_i^2-(\sum_{i=1}^nx_i)^2$ 半正定



## 17.

$Ax=0 \Rightarrow A^TAx=0 \Rightarrow x^TA^TAx=0$

$x^TA^TAx=0 \Rightarrow (Ax)^TAx=0 \Rightarrow Ax=0 \Rightarrow A^TAx=0$

$\therefore Ax=0$ 与 $A^TAx=0$ 有相同的解, 根据其基础解系的性质可知

$\therefore n - \text{rank}(A) = n - \text{rank}(A^TA)$

$\therefore \text{rank}(A)=\text{rank}(A^TA)$