# P268. 1. 2.

## 1.

已知 $M\subseteq N$, 即 $\forall x, x\in M\rightarrow x\in N \equiv T \Leftrightarrow \lnot x\in M\lor x\in N\equiv T$

$
\begin{aligned}
\therefore M
&=\{x|x\in M\} \\
&=\{x|x\in M \land (\lnot x\in M\lor x\in N)\} \\
&=\{x|x\in M \land \lnot x\in M\lor x\in M \land x\in N\} \\
&=\{x|x\in M \land x\in N\} \\
&=M\cap N \\
\end{aligned}
$

$
\begin{aligned}
\therefore N
&=\{x|x\in N\} \\
&=\{x|x\in N \lor \lnot(\lnot x\in M\lor x\in N)\} \\
&=\{x|x\in N \lor ( x\in M\land \lnot x\in N)\} \\
&=\{x|(x\in N \lor  x\in M)\land (x\in N \lor\lnot x\in N)\} \\
&=\{x|x\in M \lor x\in N\} \\
&=M\cup N \\
\end{aligned}
$


## 2.

$
\begin{aligned}
\therefore M\cap (N\cup L)
&=\{x|x\in M \land (x\in N \lor x\in L)\} \\
&=\{x|x\in M \land x\in N \lor x\in M \land x\in L\} \\
&=(M\cap N)\cup(M\cap L) \\
\end{aligned}
$

$
\begin{aligned}
\therefore M\cup (N\cap L)
&=\{x|x\in M \lor (x\in N \land x\in L)\} \\
&=\{x|(x\in M \lor x\in N) \land (x\in M \lor x\in L)\} \\
&=(M\cup N)\cap(M\cup L) \\
\end{aligned}
$

