# 五.

$对于n=2时, D_2=x^2+xy+y^2$

$对于n时, 假设D_{n-1}=\displaystyle\sum_{k=0}^{n-1}x^{n-k}y^k$

$$
\begin{aligned}
&
\begin{vmatrix}
x+y &xy &0 &\cdots &0 \\
1 &x+y &xy &\cdots &0 \\
0 &1 &x+y &\cdots &0 \\
\vdots &\vdots &\vdots & &\vdots \\
0 &0 &0 &\cdots &x+y \\
\end{vmatrix}
\\ =&
\begin{vmatrix}
x &xy &0 &\cdots &0 \\
1 &x+y &xy &\cdots &0 \\
0 &1 &x+y &\cdots &0 \\
\vdots &\vdots &\vdots & &\vdots \\
0 &0 &0 &\cdots &x+y \\
\end{vmatrix}
+
\begin{vmatrix}
y &xy &0 &\cdots &0 \\
0 &x+y &xy &\cdots &0 \\
0 &1 &x+y &\cdots &0 \\
\vdots &\vdots &\vdots & &\vdots \\
0 &0 &0 &\cdots &x+y \\
\end{vmatrix}
\\ =&
\begin{vmatrix}
x &0 &0 &\cdots &0 \\
1 &x &0 &\cdots &0 \\
0 &1 &x &\cdots &0 \\
\vdots &\vdots &\vdots & &\vdots \\
0 &0 &0 &\cdots &x \\
\end{vmatrix}
+
\begin{vmatrix}
x+y &xy &\cdots &0 \\
1 &x+y &\cdots &0 \\
\vdots &\vdots & &\vdots \\
0 &0 &\cdots &x+y \\
\end{vmatrix}
\\ =&
x^n+y\sum_{k=0}^{n-1}x^{n-k}y^k
\\ =&
\sum_{k=0}^{n}x^{n-k}y^k
\end{aligned}
$$


# 六.



---

# 离散

$n=a_1+a_2+\cdots+a_k$

$r=a_1^2+a_2^2+\cdots+a_t^2$

$(1^2+1^2+\cdots+1^2)(a_1^2+a_2^2+\cdots+a_t^2)\geq(a_1+a_2+\cdots+a_t)^2$

$\Rightarrow$

$t\cdot r\geq n^2$