$\displaystyle \frac{\mathrm{d}}{\mathrm{d}s}(-\frac{s^{2}+2s+2}{s(s+4)}) = \frac{2 (- s^{2} + 2 s + 4)}{s^{2} (s + 4)^{2}}$

$\displaystyle - s^{2} + 2 s + 4=0 = [ s = 1 - \sqrt{5}, \  s = 1 + \sqrt{5}]$

$\displaystyle K=(-\frac{s^{2}+2s+2}{s(s+4)})|_{s=1-\sqrt{5}} = - \frac{1}{4} + \frac{\sqrt{5}}{4} = 0.309016994374947$

$\frac{(s^{2}+2s+2+Ks(s+4))}{1+K}|_{K=- \frac{1}{4} + \frac{\sqrt{5}}{4}} = s^{2} + 2.47213595499958 s + 1.52786404500042 = s^{2} + 2.48 s + 1.5376$

$s^{2}+4s+5=0 = [ s = -2 - i, \  s = -2 + i]$

$\displaystyle \frac{\mathrm{d}}{\mathrm{d}s}(-\frac{s^{2}+4s+5}{s+1}) = \frac{- s^{2} - 2 s + 1}{s^{2} + 2 s + 1}$

$- s^{2} - 2 s + 1=0 = [ s = -1 + \sqrt{2}, \  s = - \sqrt{2} - 1 = -2.41421356237309]$

$\displaystyle \frac{\mathrm{d}}{\mathrm{d}s}(-\frac{s^{2}(s+9)}{s+1}) = \frac{- 2 s (s + 3)^{2}}{(s + 1)^{2}}$

$s^{2}+2s+5=0 = [ s = -1 - 2 i, \  s = -1 + 2 i]$

$\displaystyle (\arctan \frac{1}{2}) \frac{360}{2\pi} = 116.565051177078$

$180\times 3-90-117 = 333$

$\displaystyle \frac{\mathrm{d}}{\mathrm{d}s}(-\frac{s(s+1)}{s+2}) = - \frac{s^{2} + 4 s + 2}{(s + 2)^{2}}$

$\displaystyle (K(s+2)+s(s+1))|_{s=-2+j\omega} = i K \omega - \omega^{2} - 3 i \omega + 2$

---

$\displaystyle \frac{\frac{1}{(s+1)(s+2)}}{1+\frac{1}{(s+1)(s+2)}} = \frac{1}{s^{2} + 3 s + 3}$

$\omega_{n}=\sqrt{3}$, $\displaystyle \zeta = \frac{3}{2\omega_n}=0.866025403784439$ 欠阻尼.

$\displaystyle \frac{\frac{K(s+z)}{(s+1)(s+2)}}{1+\frac{K(s+z)}{(s+1)(s+2)}} = \frac{K (s + z)}{s^{2} + (K + 3)s + K z  + 2}$

$\omega_n=\sqrt{K z  + 2}$, $\displaystyle \zeta=\frac{K + 3}{2\sqrt{K z  + 2}}=(\frac{K + 3}{2\sqrt{K z  + 2}})|_{K=1}=\frac{2}{\sqrt{z + 2}}$

$\displaystyle \frac{\frac{K}{(s+1)(s+2)}}{1+\frac{K}{(s+1)(s+2)}} = \frac{K}{s^{2} + 3 s + K + 2}$

$\omega_n = \sqrt{K+2}$, $\displaystyle \zeta=\frac{3}{2\sqrt{K+2}}$

$\displaystyle \frac{\frac{Ks}{(s+1)(s+2)}}{1+\frac{Ks}{(s+1)(s+2)}} = \frac{K s}{s^{2} + (K + 3) s+ 2}$

$\omega_n = \sqrt{2}$, $\displaystyle \zeta=\frac{K+3}{2\sqrt{2}}$

$\displaystyle \frac{\frac{K \frac{1}{s}}{(s+1)(s+2)}}{1+\frac{K \frac{1}{s}}{(s+1)(s+2)}} = \frac{K}{s^{3} + 3 s^{2} + 2 s + K}$

$\omega_n = \sqrt{2}$, $\displaystyle \zeta=\frac{K+3}{2\sqrt{2}}$

---

$\displaystyle \frac{\mathrm{d}}{\mathrm{d}s}(-\frac{s^{3}}{(s+10)(s+2)}) = \frac{- s^{2} (s^{2} + 24 s + 60)}{(s + 2)^{2} (s + 10)^{2}}$

$s^{2} (s^{2} + 24 s + 60)=0 = [ s = 0, \  s = -12 - 2 \sqrt{21} = -21.1651513899117, \  s = -12 + 2 \sqrt{21}]$

$\displaystyle (-\frac{s^{3}}{(s+10)(s+2)})|_{s=-12 - 2 \sqrt{21}} = \frac{81}{4} + \frac{21 \sqrt{21}}{4} = 44.3085223985182$

$\displaystyle s\frac{1}{1+\frac{K(s+10)(s+2)}{s^{3}}}\frac{1}{s^{2}} = \frac{s^{2}}{K (s + 2) (s + 10) + s^{3}}$
