$\begin{bmatrix} 12 & 4 \\\end{bmatrix}(s \begin{bmatrix} 1 & 0 \\ 0 & 1 \\\end{bmatrix} - \begin{bmatrix} 0 & 1 \\ -12 & -8 \\\end{bmatrix})^{-1} \begin{bmatrix} 0 \\ 1\end{bmatrix} = \begin{bmatrix}\frac{4 (s + 3)}{s^{2} + 8 s + 12}\end{bmatrix}$


$\displaystyle \frac{-1}{s(s+1)^{2}} = \frac{1}{s^{2} + 2 s + 1} + \frac{1}{s + 1} - \frac{1}{s}$


$e^{At}|_{A = \begin{bmatrix} 1 & -2 \\ 2 & -3 \\\end{bmatrix}} = \begin{bmatrix}(2 t + 1) e^{- t} & - 2 t e^{- t}\\2 t e^{- t} & (1 - 2 t) e^{- t}\end{bmatrix}$

$\displaystyle \frac{6}{s(s+2)(s+3)} = \frac{2}{s + 3} - \frac{3}{s + 2} + \frac{1}{s}$

$2\times 2\times 14 + 4 \times  4 \times 32 + 4 \times 20 \times 2 = 728$

$A^{3}+3A^{2}-8A$

$(\begin{bmatrix}-8 & -5 & -3\\24 & 7 & 4\\-32 & 4 & -5\end{bmatrix}+\begin{bmatrix}0 & 0 & 3\\-24 & -15 & -9\\72 & 21 & 12\end{bmatrix}-\begin{bmatrix}0 & 8 & 0\\0 & 0 & 8\\-64 & -40 & -24\end{bmatrix}+10\begin{bmatrix} 1 & 0 & 0 \\ 0 & 1 & 0 \\ 0 & 0 & 1 \\\end{bmatrix})\begin{bmatrix} 2 & -4 & 0 \\ 0 & 2 & -4 \\ 32 & 20 & 14 \\\end{bmatrix}^{-1}\begin{pmatrix} 0 \\ 0 \\ 1 \\\end{pmatrix} = \begin{bmatrix}- \frac{9}{91}\\- \frac{9}{182}\\\frac{587}{182}\end{bmatrix} = \begin{bmatrix}-0.0989010989010989\\-0.0494505494505494\\3.22527472527473\end{bmatrix}$

$(\lambda^{2}-2\lambda+2)(\lambda+5) = \lambda^{3} + 3 \lambda^{2} - 8 \lambda + 10$
