# 概率统计第六次作业

## 201300035 方盛俊

## 6.1

要证 $\displaystyle P(X\geqslant \epsilon)=\int_{\epsilon}^{+\infty}\frac{1}{\sqrt{2\pi}}e^{-\frac{x^{2}}{2}}\mathrm{d}x\geqslant \frac{1}{3}e^{-\frac{(\epsilon+1)^{2}}{2}}$

即证 $\displaystyle \int_{\epsilon}^{+\infty}\frac{1}{\sqrt{2\pi}}e^{-\frac{x^{2}}{2}}\mathrm{d}x-\frac{1}{3}e^{-\frac{(\epsilon+1)^{2}}{2}}\geqslant 0$

令 $\displaystyle f(\epsilon)=\int_{\epsilon}^{+\infty}\frac{1}{\sqrt{2\pi}}e^{-\frac{x^{2}}{2}}\mathrm{d}x-\frac{1}{3}e^{-\frac{(\epsilon+1)^{2}}{2}}$

$\therefore \displaystyle f'(\epsilon)=\frac{1}{3}(\epsilon+1)e^{-\frac{\epsilon^{2}+2\epsilon+1}{2}}- \frac{1}{\sqrt{2\pi}}e^{- \frac{\epsilon^{2}}{2}}=e^{-\frac{\epsilon^{2}}{2}}\left[ \frac{1}{3}(\epsilon+1)e^{-\frac{1}{2}}\cdot e^{-\epsilon}-\frac{1}{\sqrt{2\pi}} \right]$

令 $\displaystyle g(\epsilon)=\frac{1}{3}(\epsilon+1)e^{-\frac{1}{2}}\cdot e^{-\epsilon}-\frac{1}{\sqrt{2\pi}}$

$\therefore \displaystyle g'(\epsilon)=-\frac{1}{3}\epsilon e^{- \epsilon - \frac{1}{2}}<0$

$\therefore \displaystyle g(\epsilon)< g(0)=\frac{1}{3}e^{-\frac{1}{2}}-\frac{1}{\sqrt{2\pi}}<0$

$\therefore f'(\epsilon)<0$

$\therefore \displaystyle f(\epsilon)\geqslant \lim_{\epsilon \to \infty}\left[ \int_{\epsilon}^{+\infty}\frac{1}{\sqrt{2\pi}}e^{-\frac{x^{2}}{2}}\mathrm{d}x-\frac{1}{3}e^{-\frac{(\epsilon+1)^{2}}{2}} \right]=0$

$\therefore \displaystyle P(X\geqslant \epsilon)\geqslant \frac{1}{3}e^{-\frac{(\epsilon+1)^{2}}{2}}$


## 6.2 

$
\begin{aligned}
E(X)
&=\int_{0}^{+\infty}\frac{x}{\beta^{\alpha}\Gamma(\alpha)}x^{\alpha-1}e^{-\frac{x}{\beta}}\mathrm{d}x \\
&=\frac{1}{\beta^{\alpha}\Gamma(\alpha)}\int_{0}^{+\infty}x^{\alpha}e^{-\frac{x}{\beta}}\mathrm{d}x \\
&=\frac{-\beta}{\beta^{\alpha}\Gamma(\alpha)}\int_{0}^{+\infty}x^{\alpha}\mathrm{d}e^{-\frac{x}{\beta}} \\
&=\frac{-\beta}{\beta^{\alpha}\Gamma(\alpha)}\left[ [x^{\alpha}e^{-\frac{x}{\beta}}]_{0}^{+\infty}-\int_{0}^{+\infty}e^{-\frac{x}{\beta}}\mathrm{d}x^{\alpha} \right] \\
&=\frac{\alpha\beta}{\Gamma(\alpha)}\int_{0}^{+\infty}(\frac{x}{\beta})^{\alpha-1}e^{-\frac{x}{\beta}}\mathrm{d}\frac{x}{\beta} \\
&=\alpha\beta
\end{aligned}
$

$
\begin{aligned}
E(X^{2})
&=\int_{0}^{+\infty}\frac{x^{2}}{\beta^{\alpha}\Gamma(\alpha)}x^{\alpha-1}e^{-\frac{x}{\beta}}\mathrm{d}x \\
&=\frac{1}{\beta^{\alpha}\Gamma(\alpha)}\int_{0}^{+\infty}x^{\alpha+1}e^{-\frac{x}{\beta}}\mathrm{d}x \\
&=\frac{-\beta}{\beta^{\alpha}\Gamma(\alpha)}\int_{0}^{+\infty}x^{\alpha+1}\mathrm{d}e^{-\frac{x}{\beta}} \\
&=\frac{\beta}{\beta^{\alpha}\Gamma(\alpha)}\int_{0}^{+\infty}e^{-\frac{x}{\beta}}\mathrm{d}x^{\alpha+1} \\
&=\frac{\beta(\alpha+1)}{\beta^{\alpha}\Gamma(\alpha)}\int_{0}^{+\infty}x^{\alpha}e^{-\frac{x}{\beta}}\mathrm{d}x \\
&=\alpha^{2}\beta^{2}+\alpha\beta^{2}
\end{aligned}
$

$\mathrm{Var}(X)=E(X^{2})-E(X)^{2}=\alpha\beta^{2}$


## 6.3

### 26.

**(1)**

$\displaystyle P(2<X\leqslant 5)=P(\frac{2-3}{2}<\frac{X-3}{2}\leqslant \frac{5-3}{2})=\Phi(1)-\Phi(-\frac{1}{2})=\Phi(1)+\Phi(\frac{1}{2})-1=0.5328$

$\displaystyle P(-4<X\leqslant 10)=P(\frac{-4-3}{2}<\frac{X-3}{2}\leqslant \frac{10-3}{2})=\Phi(\frac{7}{2})-\Phi(-\frac{7}{2})=2\Phi(\frac{7}{2})-1=0.9996$

$\displaystyle P(|X|>2)=P(\frac{X-3}{2}<\frac{-2-3}{2} \ \text{or} \ \frac{X-3}{2}>\frac{2-3}{2})=1-\Phi(-\frac{1}{2})+\Phi(-\frac{5}{2})=1+\Phi(\frac{1}{2})-\Phi(\frac{5}{2})=0.6977$

$\displaystyle P(X>3)=P(\frac{X-3}{2}>\frac{3-3}{2})=1-\Phi(0)=\Phi(0)=0.5$

**(2)**

由 (1) 知 $P(X>3)=\Phi(0)$, 且有 $\displaystyle P(X\leqslant 3)=P(\frac{X-3}{2}\leqslant \frac{3-3}{2})=\Phi(0)$

$\therefore c=3$

**(3)**

$\because \displaystyle P(X>d)\geqslant 0.9$

$\therefore \displaystyle 1-\Phi(\frac{d-3}{2})=\Phi(-\frac{d-3}{2})\geqslant 0.9=\Phi(1.282)$

$\because \Phi(x)$ 单调递增

$\therefore \displaystyle -\frac{d-3}{2}\geqslant 1.282$

$\therefore d\leqslant 0.436$


### 32.

$\because \displaystyle f(x), g(x)$ 都是概率密度函数

$\therefore \displaystyle f(x) \geqslant 0, g(x)\geqslant 0, \int_{-\infty}^{+\infty}f(x)\mathrm{d}x=1, \int_{-\infty}^{+\infty}g(x)\mathrm{d}x=1$

$\therefore h(x)=\alpha f(x)+(1-\alpha)g(x)\geqslant 0$

$\therefore \displaystyle \int_{-\infty}^{+\infty}h(x)\mathrm{d}x=\int_{-\infty}^{+\infty}[\alpha f(x)+(1-\alpha)g(x)]\mathrm{d}x=\alpha\int_{-\infty}^{+\infty}f(x)\mathrm{d}x+(1-\alpha)\int_{-\infty}^{+\infty}g(x)\mathrm{d}x=\alpha+(1-\alpha)=1$

$\therefore \displaystyle h(x)$ 是概率密度函数


### 34.

**(1)**

$\because X$ 在 $(0,1)$ 服从均匀分布

$\therefore f_{x}(x)=1, 0\leqslant x\leqslant 1$

$\therefore F_{y}(y)=P(Y\leqslant y)=P(e^{X}\leqslant y)=P(X\leqslant \ln y)=F_{x}(\ln y), 1\leqslant y\leqslant e$

$\therefore \displaystyle f_{y}(y)=f_{x}(\ln y)\cdot \frac{1}{y}=\frac{1}{y}, 1\leqslant y\leqslant e$

$\therefore f_{y}(y)=\begin{cases} \frac{1}{y}, & 1\leqslant y\leqslant e \\  0, & \text{otherwise} \end{cases}$

**(2)**

$\therefore F_{y}(y)=P(Y\leqslant y)=P(-2\ln X\leqslant y)=P(X\geqslant e^{-\frac{1}{2}y})=1-F_{x}(e^{-\frac{1}{2}y}), y\geqslant 0$

$\therefore \displaystyle f_{y}(y)=-f_{x}(e^{-\frac{1}{2}y})\cdot e^{-\frac{1}{2}y}\cdot (-\frac{1}{2})=\frac{1}{2}e^{-\frac{1}{2}y}, y\geqslant 0$

$\therefore f_{y}(y)=\begin{cases} \frac{1}{2}e^{-\frac{1}{2}y}, & y\geqslant 0 \\  0, & \text{otherwise} \end{cases}$


### 35.

**(1)**

$\because X\sim N(0,1)$

$\therefore \displaystyle f_{x}(x)=\frac{1}{\sqrt{2\pi}}e^{-\frac{x^{2}}{2}}$

$\therefore \displaystyle F_{y}(y)=P(Y\leqslant y)=P(e^{X}\leqslant y)=P(X\leqslant \ln y)=F_{x}(\ln y), y>0$

$\therefore \displaystyle f_{y}(y)=f_{x}(\ln y)\cdot \frac{1}{y}=\frac{1}{\sqrt{2\pi}y}e^{-\frac{(\ln y)^{2}}{2}}, y>0$

$\therefore \displaystyle f_{y}(y)=\begin{cases} \frac{1}{\sqrt{2\pi}y}e^{-\frac{(\ln y)^{2}}{2}}, & y>0 \\ 0, & y \leqslant 0 \end{cases}$

**(2)**

$\therefore \displaystyle F_{y}(y)=P(Y\leqslant y)=P(2X^{2}+1\leqslant y)=P(-\sqrt{\frac{y-1}{2}}\leqslant X\leqslant \sqrt{\frac{y-1}{2}})=F_{x}(\sqrt{\frac{y-1}{2}})-F_{x}(-\sqrt{\frac{y-1}{2}}), y\geqslant 1$

$\therefore \displaystyle f_{y}(y)=f_{x}(\sqrt{\frac{y-1}{2}})\cdot \frac{1}{4}\cdot (\frac{y-1}{2})^{-\frac{1}{2}}+f_{x}(-\sqrt{\frac{y-1}{2}})\cdot \frac{1}{4}\cdot (\frac{y-1}{2})^{-\frac{1}{2}}=\frac{1}{4}(\frac{y-1}{2})^{-\frac{1}{2}}\left[f_{x}(\sqrt{\frac{y-1}{2}})+f_{x}(-\sqrt{\frac{y-1}{2}})\right]=\frac{1}{2\sqrt{2\pi}}(\frac{y-1}{2})^{-\frac{1}{2}}e^{-\frac{y-1}{4}} , y\geqslant 0$

$\therefore \displaystyle f_{y}(y)=\begin{cases} \frac{1}{2\sqrt{2\pi}}(\frac{y-1}{2})^{-\frac{1}{2}}e^{-\frac{y-1}{4}}, & y\geqslant 0 \\ 0, & y < 0 \end{cases}$

**(3)**

$\therefore F_{y}(y)=P(Y\leqslant y)=P(|X|\leqslant y)=P(-y\leqslant X\leqslant y)=F_{x}(y)-F_{x}(-y), y\geqslant 0$

$\therefore \displaystyle f_{y}(y)=f_{x}(y)+f_{x}(-y)=\frac{\sqrt{2\pi}}{\pi}e^{-\frac{y^{2}}{2}}, y\geqslant 0$

$\therefore \displaystyle f_{y}(y)=\begin{cases} \frac{\sqrt{2\pi}}{\pi}e^{-\frac{y^{2}}{2}}, & y\geqslant 0 \\ 0, & y < 0 \end{cases}$


### 36.

**(1)**

$\therefore F_{y}(y)=P(Y\leqslant y)=P(X^{3}\leqslant y)=P(X\leqslant \sqrt[3]{y})=F_{x}(\sqrt[3]{y})$

$\therefore \displaystyle f_{y}(y)=\frac{1}{3}y^{-\frac{2}{3}}f(\sqrt[3]{y})$

**(2)**

$\therefore F_{y}(y)=P(Y\leqslant y)=P(X^{2}\leqslant y)=P(-\sqrt{y}\leqslant X\leqslant \sqrt{y})=F_{x}(\sqrt{y})-F_{x}(-\sqrt{y})=F_{x}(\sqrt{y}), y\geqslant 0$

$\therefore \displaystyle f_{y}(y)=\frac{1}{2}y^{-\frac{1}{2}}f(\sqrt{y})=\frac{1}{2}y^{-\frac{1}{2}}e^{-\sqrt{y}}, y\geqslant 0$

$\therefore \displaystyle f_{y}(y)=\begin{cases} \frac{1}{2}y^{-\frac{1}{2}}e^{-\sqrt{y}}, & y\geqslant 0 \\ 0, & y < 0 \end{cases}$


### 37.

$\therefore F_{y}(y)=P(Y\leqslant y)=P(\sin X\leqslant y)=P(X\leqslant \arcsin y \ \text{or} \ X\geqslant \pi-\arcsin y)=F_{x}(\arcsin y)+1-F_{x}(\pi - \arcsin y), 0<y<1$

$\therefore \displaystyle f_{y}(y)=\frac{2\arcsin y}{\pi^{2}\sqrt{1 - y^{2}}}+\frac{2(\pi-\arcsin y)}{\pi^{2}\sqrt{1-y^{2}}}=\frac{2}{\pi\sqrt{1-y^{2}}}$

$\therefore \displaystyle f_{y}(y)=\begin{cases} \frac{2}{\pi\sqrt{1-y^{2}}}, & 0<y<0 \\ 0, & \text{otherwise} \end{cases}$


## 6.4

$\because \displaystyle P(x_1<X\leqslant x_2, y_1<Y\leqslant y_2)=F(x_2,y_2)-F(x_2,y_1)-F(x_1,y_2)+F(x_1,y_1)$

$\therefore \displaystyle P(X>x, Y>y)=P(x<X\leqslant +\infty, y<Y\leqslant +\infty)=F(+\infty,+\infty)-F(+\infty,y_1)-F(x_1,+\infty)+F(x_1,y_1)=1-F(+\infty,y_1)-F(x_1,+\infty)+F(x_1,y_1)$

$\therefore \displaystyle P(X>x, Y>y)=1-F(+\infty,y_1)-F(x_1,+\infty)+F(x_1,y_1)$