# 概率统计第四次作业

## 3.1

**证明 $E(X)=np$:**

$\because X\sim B(n,p)$

$\therefore \displaystyle P(X=k)=\binom{n}{k}p^{k}(1-p)^{n-k}$

$\therefore \displaystyle E(X)=\sum_{k=0}^{\infty}k\cdot P(X=k)=\sum_{k=0}^{\infty}k\binom{n}{k}p^{k}(1-p)^{n-k}=(1-p)^{n}\sum_{k=1}^{\infty}k\binom{n}{k}\left( \frac{p}{1-p} \right)^{k}$

令 $\displaystyle x=\frac{p}{1-p}$, 则

$\because \displaystyle \sum_{k=0}^{\infty}\binom{n}{k}x^{k}=(1+x)^{n}$

两边求导得

$\therefore \displaystyle \sum_{k=1}^{\infty}k\binom{n}{k}x^{k-1}=n(1+x)^{n-1}$

$\therefore \displaystyle \sum_{k=1}^{\infty}k\binom{n}{k}x^{k}=nx(1+x)^{n-1}$

$\therefore \displaystyle E(X)=(1-p)^{n}\cdot n\cdot \frac{p}{1-p}\cdot \left( 1+\frac{p}{1-p} \right)^{n-1}=np$

**证明 $\mathrm{Var}(X)=np(1-p)$:** 

$
\begin{aligned}
\therefore \mathrm{E}(X^{2})
&=\sum_{k=0}^{\infty}k^{2}\cdot P(X=k) \\
&=\sum_{k=0}^{\infty}k^{2}\binom{n}{k}p^{k}(1-p)^{n-k} \\
&=\sum_{k=0}^{\infty}k(k-1)\binom{n}{k}p^{k}(1-p)^{n-k}+\sum_{k=0}^{\infty}k\binom{n}{k}p^{k}(1-p)^{n-k} \\
&=(1-p)^{n}\sum_{k=1}^{\infty}k(k-1)\binom{n}{k}\left( \frac{p}{1-p} \right)^{k}+(1-p)^{n}\sum_{k=1}^{\infty}k\binom{n}{k}\left( \frac{p}{1-p} \right)^{k} \\
\end{aligned}
$

$\because \displaystyle \sum_{k=1}^{\infty}k\binom{n}{k}x^{k-1}=n(1+x)^{n-1}$

$\therefore \displaystyle \sum_{k=2}^{\infty}k(k-1)\binom{n}{k}x^{k-2}=n(n-1)(1+x)^{n-2}$

$\therefore \displaystyle \sum_{k=2}^{\infty}k(k-1)\binom{n}{k}x^{k}=n(n-1)x^{2}(1+x)^{n-2}$

$\therefore \displaystyle E(X^{2})=(1-p)^{n}\cdot n(n-1)\left( \frac{p}{1-p} \right)^{2}\left( 1+\frac{p}{1-p} \right)^{n-2}+np=n(n-1)p^{2}+np=np(1-p)+n^{2}p^{2}$

$\therefore \displaystyle \mathrm{Var}(X)=E(X^{2})-E(X)^{2}=np(1-p)$


## 3.2

**证明 $\displaystyle E(X)=\frac{1}{p}$:**

$\because \displaystyle P(X=k)=(1-p)^{k-1}p$

$\therefore \displaystyle E(X)=\sum_{k=1}^{\infty}k\cdot P(X=k)=\sum_{k=1}^{\infty}k(1-p)^{k-1}p=p\sum_{k=1}^{\infty}k(1-p)^{k-1}$

$\because \displaystyle \sum_{k=0}^{\infty}x^{k}=\frac{1}{1-x}$

$\therefore \displaystyle \sum_{k=1}^{\infty}kx^{k-1}=\frac{1}{(1-x)^{2}}$

$\therefore \displaystyle \sum_{k=1}^{\infty}k(1-p)^{k-1}=\frac{1}{p^{2}}$

$\therefore \displaystyle E(X)=p\cdot \frac{1}{p^{2}}=\frac{1}{p}$

**证明 $\displaystyle \mathrm{Var}(X)=\frac{1-p}{p^{2}}$:**

$\therefore \displaystyle E(X^{2})=\sum_{k=1}^{\infty}k^{2}(1-p)^{k-1}p=p\sum_{k=2}^{\infty}k(k-1)(1-p)^{k-1}+p\sum_{k=1}^{\infty}k(1-p)^{k-1}$

$\because \displaystyle \sum_{k=1}^{\infty}kx^{k-1}=\frac{1}{(1-x)^{2}}$

$\therefore \displaystyle \sum_{k=2}^{\infty}k(k-1)x^{k-2}=\frac{2}{(1-x)^{3}}$

$\therefore \displaystyle \sum_{k=2}^{\infty}k(k-1)x^{k-1}=\frac{2x}{(1-x)^{3}}$

$\therefore \displaystyle E(X^{2})=p\cdot \frac{2(1-p)}{p^{3}}+\frac{1}{p}=\frac{1}{p}+\frac{2(1-p)}{p^{2}}=\frac{2 - p}{p^{2}}$

$\therefore \displaystyle \mathrm{Var}(X)=E(X^{2})-E(X)^{2}=\frac{2 - p}{p^{2}}-\frac{1}{p^{2}}=\frac{1 - p}{p^{2}}$


## 3.3






