# 第九次作业

10.4，10.5，11.2，11.5，11.10

## 10.4

$\because\displaystyle h=(L-R\varphi-R\tan\theta)\cos\theta$

$\therefore\displaystyle \frac{{\rm d}L}{{\rm d}T}-\frac{{\rm d}R}{{\rm d}T}\left( \frac{\pi}{2}-\theta+\tan\theta \right)$

$\therefore\displaystyle \frac{{\rm d}L}{{\rm d}T}\equiv L\alpha_{\text{steel}}, \frac{{\rm d}R}{{\rm d}T}\equiv R\alpha_{\text{Al}}$

$\therefore\displaystyle L\alpha_{\text{steel}}-R\alpha_{\text{Al}}\left( \frac{\pi}{2}-\theta+\tan\theta \right)=0$

$\therefore\displaystyle R=\frac{2L}{\pi-2\theta+2\theta}\frac{\alpha_{\text{steel}}}{\alpha_{\text{Al}}}\approx 0.63 \ \text{m}$

## 10.5

$\because\displaystyle a^2x\rho_{\text{Hg}}g=a^3\rho_{\text{Al}}g, x=a\frac{\rho_{\text{Al}}}{\rho_{\text{Hg}}}=3.97 \ \text{cm}$

同时我们有

$\displaystyle \ln x=\ln a+\ln \rho_{\text{Al}}-\ln \rho_{\text{Hg}}$

$\displaystyle \frac{{\rm d}\ln x}{{\rm d}T}=\frac{1}{a}\frac{{\rm d}a}{{\rm d}T}+\frac{1}{\rho_{\text{Al}}}\frac{{\rm d}\rho_{\text{Al}}}{{\rm d}T}-\frac{1}{\rho_{\text{Hg}}}\frac{{\rm d}\rho_{\text{Hg}}}{{\rm d}T}$

$\therefore\displaystyle \frac{1}{\rho_{\text{Al}}}\frac{{\rm d}\rho_{\text{Al}}}{{\rm d}T}=\frac{V}{m}\frac{{\rm d}}{{\rm d}T}\left( \frac{m}{V} \right)=V\left( -\frac{1}{V^2} \right)\frac{{\rm d}V}{{\rm d}T}=-\frac{1}{V}\frac{{\rm d}v}{{\rm d}t}=-\beta$

$\therefore\displaystyle \int {\rm d}\ln x=\int{\rm d}T(\alpha_{\text{Al}}-\beta_{\text{Al}}+\beta_{\text{Hg}})=(\alpha_{\text{Al}}-\beta_{\text{Al}}+\beta_{\text{Hg}})\int{\rm d}T$

$\therefore\displaystyle \ln\frac{x}{x_0}(\alpha_{\text{Al}}-\beta_{\text{Al}}+\beta_{\text{Hg}})\Delta T=6.7\times 10^{-3}$

$\therefore\displaystyle \Delta x=x_0(e^{6.7\times 10^{-3}}-1)=x_0\times6.7\times 10^{-3}=0.27\ \text{mm}$

## 11.2

$\because\displaystyle p=\frac{AT^3}{V}, U=BT^n\ln\left( \frac{V}{V_0} \right)+f(T)$

由书中 P.213 页可得到方程

$\displaystyle \left( \frac{\partial U}{\partial V} \right)_T=T\left( \frac{\partial p}{\partial T} \right)_V-p$

则可得

$\displaystyle \frac{BT^n}{V}=\frac{T\cdot 3AT^2}{V}-\frac{AT^3}{V}$

解得

$n=3, B=2A$

## 11.5

$\because\displaystyle p_1=p_0+\frac{mg}{A}$

$\therefore pV^\gamma$ 为常量

$\therefore\displaystyle \frac{{\rm d}p}{p}=-\gamma\frac{{\rm d}V}{V}=-\gamma\frac{Ax}{V_0}$

$\therefore\displaystyle f={\rm d}p\cdot A=-\gamma\frac{pA^2}{V_0}x$

$\therefore\displaystyle \omega^2=\frac{\gamma A^2p}{mV_0}, v=\frac{\omega}{2\pi}$

## 11.10

$\displaystyle \eta=1-\left( \frac{V_1}{v_2} \right)^{\gamma-1}=1-\left( \frac{V_1}{v_2} \right)^{\frac{2}{5}}$